---
title: "Short_ODE_for 3State"
format: html
---

###Model Structure

We assume:

* States 1 and 2 are transient.
* State 3 is absorbing.
* Generator matrix ùëÑ has the form:


$$Q = 
\begin{bmatrix}
- (q_{12} + q_{13}) & q_{12} & q_{13} \\
q_{21} & - (q_{21} + q_{23}) & q_{23} \\
0 & 0 & 0
\end{bmatrix}$$


Let:

$$\begin{align*}
\alpha &= q_{12} + q_{13} \\
\beta  &= q_{21} + q_{23} \\
\delta &= \sqrt{(\alpha - \beta)^2 + 4 q_{12} q_{21}} \\
\lambda_1 &= \frac{- (\alpha + \beta) + \delta}{2} \\
\lambda_2 &= \frac{- (\alpha + \beta) - \delta}{2}
\end{align*}$$




The transition propabilities from state 1 are:

$$\begin{align*}
P_{11}(t) &= \left( \frac{\lambda_1 + \alpha}{\lambda_1 - \lambda_2} \right) e^{\lambda_2 t}
+ \left( \frac{\lambda_2 + \alpha}{\lambda_2 - \lambda_1} \right) e^{\lambda_1 t} \\
P_{12}(t) &= \frac{q_{12}}{\lambda_1 - \lambda_2} \left( e^{\lambda_1 t} - e^{\lambda_2 t} \right) \\
P_{13}(t) &= 1 - P_{11}(t) - P_{12}(t)
\end{align*}$$




The transition probabilities from state 2 are:

$$\begin{align*}
P_{21}(t) &= \frac{q_{21}}{\lambda_1 - \lambda_2} \left( e^{\lambda_1 t} - e^{\lambda_2 t} \right) \\
P_{22}(t) &= \left( \frac{\lambda_1 + \beta}{\lambda_1 - \lambda_2} \right) e^{\lambda_2 t}
+ \left( \frac{\lambda_2 + \beta}{\lambda_2 - \lambda_1} \right) e^{\lambda_1 t} \\
P_{23}(t) &= 1 - P_{21}(t) - P_{22}(t)
\end{align*}$$




The transition probabilities from the absorbing state 3 are:


$$\begin{align*}
P_{31}(t) &= 0 \\
P_{32}(t) &= 0 \\
P_{33}(t) &= 1
\end{align*}$$





The full transition probability matrix is:

$$P(t) = 
\begin{bmatrix}
P_{11}(t) & P_{12}(t) & P_{13}(t) \\
P_{21}(t) & P_{22}(t) & P_{23}(t) \\
0         & 0         & 1
\end{bmatrix}$$